continue proof

extract/main.ml
@@ -19,6 +19,7 @@ let main () =
       Example2.example_block_1;
       Example3.example_block_1;
       Example4.example_block_1;
+      Example5.example_block_1;
     ]
 ;;
 
